EvmAbi/ABI.lean
@@ -51,6 +51,50 @@ def abiSize : ABIType → Nat
   | .array e _ => 1 + abiSize e
   | .tuple es => 1 + es.foldl (fun acc t => acc + abiSize t) 0
 
+theorem foldl_add_eq (a : Nat) : ∀ (xs : List ABIType),
+    xs.foldl (fun acc t => acc + abiSize t) a = a + xs.foldl (fun acc t => acc + abiSize t) 0
+  | [] => by simp
+  | x :: xs => by
+    simp
+    rw [foldl_add_eq (a + abiSize x) xs, foldl_add_eq (abiSize x) xs]
+    omega
+
+theorem le_foldl_add (a : Nat) : ∀ (xs : List ABIType), a ≤ xs.foldl (fun acc t => acc + abiSize t) a
+  | [] => Nat.le_refl a
+  | x :: xs => by
+    simp
+    have h' : a + abiSize x ≤ xs.foldl (fun acc t => acc + abiSize t) (a + abiSize x) :=
+      le_foldl_add (a + abiSize x) xs
+    exact Nat.le_trans (Nat.le_add_right a (abiSize x)) h'
+
+theorem mem_foldl_le (t : ABIType) (ts : List ABIType) (h : t ∈ ts) :
+    abiSize t ≤ ts.foldl (fun acc t => acc + abiSize t) 0 := by
+  induction ts with
+  | nil => simp at h
+  | cons x xs ih =>
+    simp at h
+    cases h with
+    | inl h_eq =>
+      rw [h_eq]
+      simp
+      exact le_foldl_add (abiSize x) xs
+    | inr h_mem =>
+      have h_ih := ih h_mem
+      refine Nat.le_trans h_ih ?_
+      simp
+      rw [foldl_add_eq (abiSize x) xs, foldl_add_eq 0 xs]
+      omega
+
+theorem abiSize_lt_array (e : ABIType) (s : Option Nat) : abiSize e < abiSize (.array e s) := by
+  simp [abiSize]
+
+theorem abiSize_lt_tuple (t : ABIType) (ts : List ABIType) (h : t ∈ ts) : abiSize t < abiSize (.tuple ts) := by
+  simp [abiSize]
+  have hle : abiSize t ≤ ts.foldl (fun acc t => acc + abiSize t) 0 :=
+    mem_foldl_le t ts h
+  apply Nat.lt_of_le_of_lt hle
+  omega
+
 def roundUp32 (n : Nat) : Nat := ((n + 31) / 32) * 32
 
 def zeroByte : UInt8 := 0
